src/polyfix.lean
@@ -1,14 +1,15 @@
 import polycodable
 import npolynomial
 
-variables {α β : Type*}
+variables {α β : Type}
 
 open part_eval (eval time_iter)
+open polycodable (encode decode)
 
 lemma pfun.res_mono (f : α →. β) {S S' : set α} {x y} (h : y ∈ f.res_inter S x) (hS : S ⊆ S') : y ∈ f.res_inter S' x :=
 by { simp at h ⊢, tauto, }
 
-theorem time_bound_fix {c : code} {b₁ b₂ b₃ : ℕ → ℕ} (mb : monotone b₁) 
+theorem time_bound_fix {c : code} (b₁ b₂ b₃ : ℕ → ℕ) (mb : monotone b₁) 
   (h₁ : time_bound c b₁) (h₂ : ∀ x : ptree, ∃ t ≤ b₃ x.sizeof, t ∈ (time_iter ((c.eval.map ptree.to_option).res_inter {s | s.sizeof ≤ b₂ x.sizeof}) (pfun.pure 1) x)) :
   time_bound c.fix (λ t, (b₃ t) * (b₁ (b₂ t)) + t) :=
 begin
@@ -21,273 +22,51 @@ begin
   refine (time_bound_spec h₁ hk).trans _, apply mb, exact hs,
 end
 
-
-
-#exit
-
-def fix_bounded_while (f : α → β ⊕ α) (P : α → Prop) [decidable_pred P] : ℕ → α → option β
-| 0 x := none
-| (n + 1) x := if P x then match f x with
-  | (sum.inl y) := some y
-  | (sum.inr x') := fix_bounded_while n x'
-end else none
-
-def fix_bounded_terminates (f : α → β ⊕ α) (P : α → Prop) [decidable_pred P] (i : ℕ) (x : α) : Prop :=
-(fix_bounded_while f P i x).is_some
-
-lemma not_fix_bounded_terminates_zero (f : α → β ⊕ α) (P : α → Prop) [decidable_pred P] (x : α) :
-  ¬fix_bounded_terminates f P 0 x := by trivial
-
-@[simp] lemma fix_bounded_terminates_iff (f : α → β ⊕ α) (P : α → Prop) [decidable_pred P] (i : ℕ) (x : α) :
-  (fix_bounded_terminates f P (i+1) x) ↔ P x ∧ (∀ x', f x = sum.inr x' → fix_bounded_terminates f P i x') :=
+theorem polytime_fix {c : code} (pc : polytime c) (p q : polynomial ℕ) (he : ∀ x : ptree, ∃ t ≤ p.eval x.sizeof, t ∈ time_iter ((c.eval.map ptree.to_option).res_inter {s | s.sizeof ≤ q.eval x.sizeof}) (pfun.pure 1) x) :
+  polytime c.fix :=
 begin
-  simp only [fix_bounded_terminates, fix_bounded_while],
-  split_ifs with H, swap, { simp [H], },
-  cases hf : f x; simp [fix_bounded_while, H],
+  rcases pc with ⟨f, f_le⟩, use p * (f.comp q) + polynomial.monomial 1 1, simp,
+  exact time_bound_fix (λ n, f.eval n) (λ n, q.eval n) (λ n, p.eval n) (monotone_polynomial_nat _) f_le he,
 end
 
-private lemma fix_bounded_while_weaken_prop {f : α → β ⊕ α} {P Q : α → Prop} {n : ℕ} {x₀ : α} {y : β} [decidable_pred P] [decidable_pred Q]
-  (h : ∀ x, P x → Q x) (hb : y ∈ fix_bounded_while f P n x₀) : y ∈ fix_bounded_while f Q n x₀ :=
+theorem code.fix_respects [polycodable α] (c : code) (f : α →. option α) (sc : ∀ x, c.eval x = (f (decode x)).map encode) :
+  part_eval.fcommutes f (c.eval.map ptree.to_option) encode :=
+{ dom_of_dom := λ x, by { specialize sc (encode x), apply_fun part.dom at sc, simp at sc, simp [sc, pfun.map], },
+  some_of_some := λ a b h, by { specialize sc (encode a), simp [pfun.map, sc, part.eq_some_iff.mpr h, encode], },
+  none_of_none := λ a h, by { specialize sc (encode a), simp [pfun.map, sc, part.eq_some_iff.mpr h, encode], } }
+
+theorem code.fix_respects' [polycodable α] (c : code) (f : α →. option α) (sc : ∀ x, c.eval x = (f (decode x)).map encode) :
+  part_eval.fcommutes (c.eval.map ptree.to_option) f decode :=
+{ dom_of_dom := λ x, by { specialize sc x, apply_fun part.dom at sc, simp at sc, simp [sc, pfun.map], },
+  some_of_some := λ a b h, by { specialize sc a, simp [pfun.map, sc] at h, rcases h with ⟨a', h₁, h₂, rfl⟩, cases a', { contradiction, }, simpa [encode, ptree.of_option], },
+  none_of_none := λ a h, by { specialize sc a, simp [pfun.map, sc] at h, rcases h with ⟨a', h₁, h₂⟩, cases a', assumption, { contradiction, },  } }
+
+lemma polytime.bdd_size_decode_encode (α : Type*) [polycodable α] :
+  ∃ (p : polynomial ℕ), ∀ x, (encode (decode x : α)).sizeof ≤ p.eval x.sizeof :=
 begin
-  induction n with n ih generalizing x₀,
-  { contradiction, },
-  simp [fix_bounded_while] at ⊢ hb, 
-  split_ifs at hb with H, swap, { contradiction, }, simp [h _ H],
-  cases (f x₀) with v; simp [fix_bounded_while] at ⊢ hb,
-  { assumption, }, { exact ih hb, },
+  obtain ⟨c, ⟨p, hp⟩, sc⟩ := polycodable.polytime_decode α, use p,
+  intro x, specialize sc x, specialize hp x, rcases hp with ⟨t, H, t_le⟩,
+  have := eval_sizeof_le_time (part.eq_some_iff.mp sc) H, exact this.trans t_le,
 end
 
-private lemma fix_bounded_while_weaken_ind {f : α → β ⊕ α} {P : α → Prop} {m n : ℕ} {x₀ : α} {y : β} [decidable_pred P]
-  (hmn : m ≤ n) (hb : y ∈ fix_bounded_while f P m x₀) : y ∈ fix_bounded_while f P n x₀ :=
+theorem polytime_fun.eval [polycodable α] {f : α → option α} {g : α → α} (hf : polytime_fun f) (p q : polynomial ℕ)
+  (hg : ∀ x, g x ∈ eval (f : α →. option α) x) (H : ∀ x : α, ∃ t ≤ p.eval (encode x).sizeof, t ∈ time_iter (pfun.res f {s : α | (encode s).sizeof ≤ q.eval (encode x).sizeof}) (pfun.pure 1) x) :
+  polytime_fun g :=
 begin
-  induction n with n ih generalizing m x₀,
-  { simp at hmn, subst hmn, contradiction, },
-  cases m, { contradiction, },
-  rw nat.succ_le_succ_iff at hmn,
-  simp [fix_bounded_while] at ⊢ hb,
-  split_ifs at ⊢ hb, swap, { contradiction, },
-  cases (f x₀) with v; simp [fix_bounded_while] at ⊢ hb,
-  { assumption, }, { exact ih hmn hb, }
+  rw polytime_fun_iff at hf, rcases hf with ⟨c, pc, sc⟩,
+  use c.fix, split, swap,
+  { intro x, simp, have := part_eval.frespects.eval_eq (c.fix_respects (f : α →. option α) _).to_frespects,
+    simp [this, part.eq_some_iff.mpr (hg x)], simp [sc], },
+  obtain ⟨P, hP⟩ := polytime.bdd_size_decode_encode α,
+  apply polytime_fix pc (p.comp P) ((q.comp P) + polynomial.monomial 1 1),
+  intro x, rcases H (decode x) with ⟨t, ht, t_mem⟩, refine ⟨t, ht.trans _, _⟩,
+  { simp, apply monotone_polynomial_nat, apply hP, },
+  have := code.fix_respects' c (f : α →. option α) _, swap, { simp [sc], }, 
+  have T := λ S : set α, part_eval.eq_time_of_fcommutes (this.restrict S), simp at T, rw ← T at t_mem,
+  rw part_eval.time_iter_invariant ({x} ∪ set.range (@encode α _)) at t_mem, simp at t_mem,
+  apply part_eval.time_iter_mono _ t_mem,
+  { intros x' y', simp, refine λ h₁ h₂ h₃, ⟨_, h₃⟩, rcases h₂ with rfl|⟨y, rfl⟩, { simp, },
+    simp at h₁, apply le_add_right, refine h₁.trans _, apply monotone_polynomial_nat, apply hP, },
+  { intros x' y' _, simp [sc, pfun.map], intros _ H₃, right, simp [encode] at H₃, rcases H₃ with ⟨y₂, _, rfl⟩, use y₂, },
+  simp,
 end
-
-lemma fix_bounded_while_weaken {f : α → β ⊕ α} {P Q : α → Prop} {m n : ℕ} {x₀ : α} {y : β} [decidable_pred P] [decidable_pred Q]
-  (hp : ∀ x, P x → Q x) (hmn : m ≤ n) (hb : y ∈ fix_bounded_while f P m x₀) : y ∈ fix_bounded_while f Q n x₀ :=
-fix_bounded_while_weaken_ind hmn (fix_bounded_while_weaken_prop hp hb)
-
-lemma fix_bounded_terminates_weaken {f : α → β ⊕ α} {P Q : α → Prop} {m n : ℕ} {x₀ : α} [decidable_pred P] [decidable_pred Q]
-  (hp : ∀ x, P x → Q x) (hmn : m ≤ n) (hb : fix_bounded_terminates f P m x₀) : fix_bounded_terminates f Q n x₀ :=
-begin
-  simp only [fix_bounded_terminates, option.is_some_iff_exists] at ⊢ hb,
-  rcases hb with ⟨y, hy⟩, use y, exact fix_bounded_while_weaken hp hmn hy,
-end
-
-lemma fix_eq_fix_bounded {f : α → β ⊕ α} {P : α → Prop} [decidable_pred P] {x : α} {y : β} {i : ℕ}
-  (h : y ∈ fix_bounded_while f P i x) : y ∈ pfun.fix (f : α →. β ⊕ α) x :=
-begin
-  induction i with i ih generalizing x,
-  { simp [fix_bounded_while] at h, contradiction, },
-  simp only [fix_bounded_while] at h, split_ifs at h with _, swap, { trivial, },
-  cases H : f x with vl vr,
-  { apply pfun.fix_stop, simp [fix_bounded_while, H] at h ⊢, exact h.symm, },
-  specialize ih (by simpa [fix_bounded_while, H, ← option.mem_def] using h),
-  rw [@comm _ (=), ← part.mem_some_iff, ← pfun.coe_val] at H,
-  rwa pfun.fix_fwd _ _ H,
-end
-
-lemma dom_of_fix_bounded_terminates {f : α → β ⊕ α} {P : α → Prop} [decidable_pred P] {x : α} {i : ℕ}
-  (h : fix_bounded_terminates f P i x) : (pfun.fix (f : α →. β ⊕ α) x).dom :=
-begin
-  rw [fix_bounded_terminates, option.is_some_iff_exists] at h, rcases h with ⟨y, hy⟩,
-  rw part.dom_iff_mem, use [y, fix_eq_fix_bounded hy],
-end
-
-section poly
-variables [polycodable α] [polycodable β]
-open polycodable (encode)
-
-lemma frespects_once_code_fix_pfun_fix {f : α →. β ⊕ α} {c : code} (hfc : ∀ x, c.eval (encode x) =  (f x).map encode) :
-  pfun.frespects_once' f (eval_fix_fun c) encode encode :=
-begin
-  intro a, split,
-  { intro h, simpa [eval_fix_fun, hfc] using h, }, split,
-  { intros a' ha', simp only [eval_fix_fun, part.mem_map_iff],
-    use (encode (ff, a')), split,
-    { rw ← part.eq_some_iff at ha', simp [hfc, ha'], refl, }, split, },
-  intros b hb, simp [eval_fix_fun], use encode (tt, b), split,
-  { rw ← part.eq_some_iff at hb, simp [hfc, hb], refl, }, split; refl,
-end
-
-lemma code_fix_eq_pfun_fix {f : α →. β ⊕ α} {c : code} (hfc : ∀ x, c.eval (encode x) =  (f x).map encode) (x : α) :
-  c.fix.eval (encode x) = (pfun.fix f x).map encode :=
-(pfun.eq_val_of_frespects_once' (frespects_once_code_fix_pfun_fix hfc) x).symm
-
-lemma code_fix_eq_pfun_fix' {f : α → β ⊕ α} {c : code} (hfc : ∀ x, c.eval (encode x) = part.some (encode $ f x)) (x : α) :
-  c.fix.eval (encode x) = (pfun.fix (f : α →. β ⊕ α) x).map encode :=
-by { apply code_fix_eq_pfun_fix, simp [hfc], }
-
-lemma eval_fix_fun_dom_eq_dom {c : code} : pfun.dom (eval_fix_fun c) = c.eval.dom :=
-by simp [pfun.dom]
-
-abbreviation encode_sizeof (x : α) := (encode x).sizeof
-
-section time_bound_fix_lemma
-
-lemma part.get_iff_mem_prop {δ : Type*} (x : part δ) (h : x.dom) (P : δ → Prop) :
-  P (x.get h) ↔ ∃ v ∈ x, P v :=
-by { split, { intro H, use x.get h, exact ⟨part.get_mem _, H⟩, }, rintro ⟨v, hv, hP⟩, rwa part.get_eq_of_mem hv h, }
-
-lemma time_bound_of_fix_bounded_terminates {c : code} {x : ptree}
-  (hc : c.eval.dom = set.univ) {T J : ℕ}
-  (ht : fix_bounded_terminates (pfun.to_fun (eval_fix_fun c) (by rwa eval_fix_fun_dom_eq_dom))
-    (λ x', (c.time.to_fun (by rwa time_dom_eq_eval_dom) x') ≤ T) J x) :
-  ∃ t ∈ c.fix.time x, t ≤ J * T + 1 :=
-begin
-  induction J with j ih generalizing x,
-  { exfalso, exact not_fix_bounded_terminates_zero _ _ _ ht, },
-  have : (c.fix.time x).dom,
-  { rw [time_dom_iff_eval_dom, code_fix_eval], simpa using dom_of_fix_bounded_terminates ht,},
-  rw part.dom_iff_mem at this, cases this with t H, use [t, H],
-  rw fix_bounded_terminates_iff at ht, cases ht with ht₁ ht₂,
-  cases fv : pfun.to_fun (eval_fix_fun c) (by rwa eval_fix_fun_dom_eq_dom) x with y x',
-  all_goals
-  { simp [pfun.to_fun, code_fix_time] at H,
-    rcases H with ⟨t', ht', rfl⟩,
-    have ht₁' : ∃ t₁ ∈ c.time x, t₁ ≤ T := by { rw ← part.get_iff_mem_prop, exact ht₁, },
-    clear ht₁, rcases ht₁' with ⟨t₁, ht₁, t₁_le⟩,
-    simp only [add_le_add_iff_right], },
-  { clear ih ht₂, simp [pfun.to_fun, eval_fix_fun] at fv, cases fv with fv₁ fv₂,
-    have : (c.eval x).dom, { change x ∈ c.eval.dom, rw hc, trivial, }, rw part.dom_iff_mem at this, cases this with fv hfv,
-    rw part.get_eq_of_mem hfv _ at fv₁ fv₂,
-    have : sum.inl t₁ ∈ time_fix_fun c (x, 0),
-    { simp [time_fix_fun], use [t₁, ht₁, fv, hfv], simp [fv₁], },
-    cases part.mem_unique (pfun.fix_stop _ this) ht', refine t₁_le.trans _, rw nat.succ_eq_add_one, nlinarith only, },
-  specialize ht₂ _ fv, specialize ih ht₂,
-  simp [pfun.to_fun, eval_fix_fun] at fv, cases fv with fv₁ fv₂,
-  have : (c.eval x).dom, { change x ∈ c.eval.dom, rw hc, trivial, }, rw part.dom_iff_mem at this, cases this with fv hfv,
-  rw part.get_eq_of_mem hfv _ at fv₁ fv₂,
-  have := time_fix_spec hfv fv₁ ht₁, subst fv₂, rw code_fix_time at this,
-  rw ← part.eq_some_iff at ht', rw [ht', @comm _ (=)] at this, simp [part.eq_some_iff] at this,
-  rcases this with ⟨t, ht, Ht⟩, rcases ih with ⟨t, ht₂, Ht₂⟩, cases part.mem_unique ht ht₂,
-  suffices : t' + 1 ≤ j * T + T + 1, { simpa [nat.succ_mul] using this, },
-  rw ← Ht, nlinarith only [Ht₂, t₁_le],
-end
-
-lemma time_bound_fix {c : code} {b₁ b₂ m : ℕ → ℕ} (hb₁ : time_bound c b₁) (mono₁ : monotone b₁) (mono₂ : monotone b₂) (mono₃ : monotone m)
-  (hb₂ : ∀ x : ptree, fix_bounded_terminates
-    (pfun.to_fun (eval_fix_fun c) (by rw [eval_fix_fun_dom_eq_dom, eval_dom_of_time_bound hb₁]))
-    (λ x', x'.sizeof ≤ m x.sizeof)
-    (b₂ x.sizeof) x) :
-  time_bound c.fix (λ t, (b₁ (m t)) * (b₂ t) + 1) :=
-begin
-  intros n v hnv, specialize hb₂ v, dsimp only, rw mul_comm,
-  apply time_bound_of_fix_bounded_terminates, swap, { rw [eval_dom_of_time_bound hb₁], },
-  refine fix_bounded_terminates_weaken _ (mono₂ hnv) hb₂,
-  intros x hx, specialize hb₁ (m v.sizeof) _ hx, rcases hb₁ with ⟨t, H, ht⟩, 
-  rw ← part.eq_some_iff at H,
-  simp [pfun.to_fun, H], exact ht.trans (mono₁ (mono₃ hnv)),
-end
-
-end time_bound_fix_lemma
-
--- TODO: This is currently very ugly
-lemma fix_bounded_terminates_norm_code_aux {f : α → β ⊕ α} {c : code} (hc : ∀ x : α, c.eval (encode x) = part.some (encode $ f x)) (hd : c.eval.dom = set.univ)
-  (P : ptree → Prop) [decidable_pred P] (i : ℕ) (x : α) :
-  fix_bounded_terminates (pfun.to_fun (eval_fix_fun c) (by rw [eval_fix_fun_dom_eq_dom, hd])) P i (encode x) ↔
-  fix_bounded_terminates f (λ y, P (encode y)) i x :=
-begin
-  induction i with i ih generalizing x, { split; intro; contradiction, },
-  simp [fix_bounded_terminates_iff], intro _,
-  split,
-  { intros h x' hx', specialize h (encode x') _, 
-    { simp [pfun.to_fun, hc, hx'], split; trivial, },
-    exact (ih x').mp h, },
-  { intros h x' hx', simp [pfun.to_fun, hc] at hx',
-    cases H : f x with val, { exfalso, cases hx' with l, rw H at l, contradiction, },
-    rw H at hx', have : x' = encode val := hx'.2, subst this,
-    rw ih, exact h _ H, }
-end
-
-lemma fix_bounded_terminates_norm_code {f : α → β ⊕ α} (hf : polytime_fun f) (P : ptree → ptree → Prop) [decidable_rel P] (i : ptree → ℕ) 
-  (start₀ : ∀ x, P x x) (start₁ : ∀ x, 0 < i x) :
-  (∀ (x : ptree), fix_bounded_terminates (pfun.to_fun (eval_fix_fun hf.norm_code) (by rw [eval_fix_fun_dom_eq_dom, hf.norm_code_dom])) (P x) (i x) x) ↔
-  ∀ (x : α), fix_bounded_terminates f (λ y, P (encode x) (encode y)) (i (encode x)) x :=
-begin
-  split,
-  { intros h x, rw ← fix_bounded_terminates_norm_code_aux hf.norm_code_eval, { exact h _, }, },
-  intros h x,
-  by_cases H : x ∈ set.range (@encode α _),
-  { rcases H with ⟨v, rfl⟩, rw fix_bounded_terminates_norm_code_aux hf.norm_code_eval, exact h _, },
-  specialize start₀ x, specialize start₁ x, cases (i x), { exfalso, simpa using start₁, },
-  rw fix_bounded_terminates_iff, refine ⟨start₀, _⟩,
-  intros x' h₂, exfalso, simpa [pfun.to_fun, hf.norm_code_invalid H] using h₂,
-end
-
-lemma polytime_fix_bounded_aux (p q : polynomial ℕ) (hpq₀ : ∀ n, 0 < p.eval n) (hpq₁ : ∀ n, n ≤ q.eval n) (f : α → β ⊕ α) (g : α → β)
-  (hg : ∀ x, g x ∈ fix_bounded_while f (λ x' : α, encode_sizeof x' ≤ q.eval (encode_sizeof x)) (p.eval (encode_sizeof x)) x)
-  (hf : polytime_fun f) : polytime_fun g :=
-begin
-  use code.fix hf.norm_code, split, swap,
-  { intro x, simp only [part.eq_some_iff, ite_eval], rw code_fix_eq_pfun_fix' hf.norm_code_eval, simpa using fix_eq_fix_bounded (hg x), },
-  rcases hf.polytime_norm_code with ⟨pc, hpc⟩,
-  use (pc.comp q) * p + 1,
-  { simp,
-    apply time_bound_fix hpc (monotone_polynomial_nat pc) (monotone_polynomial_nat p) (monotone_polynomial_nat q),
-    rw fix_bounded_terminates_norm_code hf, 
-    { intro x, simp only [fix_bounded_terminates, option.is_some_iff_exists], use (g x),
-      exact hg x, },
-    { intro x, apply hpq₁, },
-    intro, apply hpq₀, },
-end
-
-lemma polytime_fix_bounded (p q : polynomial ℕ) (f : α → β ⊕ α) (g : α → β)
-  (hg : ∀ x, g x ∈ fix_bounded_while f (λ x' : α, encode_sizeof x' ≤ q.eval (encode_sizeof x)) (p.eval (encode_sizeof x)) x)
-  (hf : polytime_fun f) : polytime_fun g :=
-begin
-  apply polytime_fix_bounded_aux (p+1) (q+polynomial.monomial 1 1) _ _ f g _ hf,
-  { intro n, simp, },
-  { intro n, simp, },
-  intro x, apply fix_bounded_while_weaken _ _ (hg x),
-  { intros x h, refine h.trans _, simp, },
-  { simp, },
-end
-
-open_locale classical
-
-lemma fix_bounded_while_with_state {γ : Type*} (f : γ → α → β ⊕ α) (P : α → Prop) (state : γ) (start : α) (n : ℕ) :
-  fix_bounded_while (f state) P n start = 
-  @fix_bounded_while _ _ (λ x : γ × α, (f x.1 x.2).map id (prod.mk x.1)) (λ x, x.1 = state ∧ P x.2) (classical.dec_pred _) n (state, start) :=
-begin
-  induction n with n ih generalizing start,
-  { simp [fix_bounded_while], },
-  by_cases H₁ : P start,
-  { cases H₂ : f state start with val; simp [fix_bounded_while, H₁, H₂, ih], },
-  { simp [fix_bounded_while, H₁], },
-end
-
-lemma polycodable.encode_tuple (x : α) (y : β) :
-  encode (x, y) = ptree.node (encode x) (encode y) := rfl
-
-@[simp] lemma encode_sizeof_tuple (x : α) (y : β) :
-  encode_sizeof (x, y) = 1 + encode_sizeof x + encode_sizeof y :=
-by { dunfold encode_sizeof, simp [polycodable.encode_tuple], }
-
-lemma polytime_fix_bounded' {δ : Type*} [polycodable δ]
-  (p q : polynomial ℕ) (f : δ → α → β ⊕ α) (g : δ → α → β)
-  (hg : ∀ d x, g d x ∈ fix_bounded_while (f d) (λ x' : α, encode_sizeof x' ≤ q.eval (encode_sizeof (d, x))) (p.eval (encode_sizeof (d, x))) x)
-  (hf : polytime_fun₂ f) : polytime_fun₂ g :=
-begin
-  classical,
-  apply polytime_fix_bounded p (q+polynomial.monomial 1 1) (λ x : δ × α, (f x.1 x.2).map id (prod.mk x.1)), swap,
-  { apply polytime_fun.sum_map, exact hf, apply polytime_fun.prod_snd, apply polytime_fun.pair, apply polytime_fun.comp polytime_fun.prod_fst polytime_fun.prod_fst, apply polytime_fun.prod_snd, },
-  rintro ⟨d, x⟩, simp only [function.uncurry_apply_pair], specialize hg d x,
-  apply fix_bounded_while_weaken,
-  rotate 2,
-  { rw ← fix_bounded_while_with_state f (λ x', encode_sizeof x' ≤ q.eval (encode_sizeof (d, x))) d x (p.eval (encode_sizeof (d, x))),
-    convert hg, },
-  { clear hg, rintro ⟨d', x'⟩ ⟨rfl, hx⟩, simp at hx ⊢, 
-    conv_rhs { rw add_comm, rw add_assoc, }, simp, apply le_add_of_nonneg_of_le, exact zero_le',
-    exact hx.trans rfl.le, },
-  { refl, },
-end
-
-end poly
